% $Id$

\documentclass[a4paper,12pt]{article}
\usepackage{amssymb}
\usepackage{pst-all}
\usepackage{lscape}

\setlength{\parindent}{0mm}
\setlength{\parskip}{7.5mm}

\newcommand{\nonterminal}[1]{$\langle #1 \rangle$}

\begin{document}

\title{Course 3BA7: Compiler Design I \\ Additional Lecture Notes \\ $2^{nd}$ November 2004}

\maketitle

\section*{A Grammar for Arithmetic Expressions}

\subsection*{Productions}

\begin{eqnarray}
\langle E \rangle		&	\to	&	\langle T \rangle		\\
\langle E \rangle		&	\to	&	\langle T \rangle		\\
\langle T \rangle		&	\to	&	\langle T \rangle \ast \langle P \rangle \\
\langle T \rangle		&	\to	&	\langle P \rangle \\
\langle P \rangle		&	\to	&	\left( \langle E \rangle \right) \\
\langle P \rangle		&	\to	&	CONST
\end{eqnarray}

This is the $\langle E \rangle + \langle T \rangle$ grammar.

$\langle E \rangle$ is an Expression. \\
$\langle T \rangle$ is a Term. \\
$\langle F \rangle$ is a Factor (not shown). \\
$\langle P \rangle$ is a Primary.


Given this grammar, we should be able to derive the expression $1 + 2
\ast 3 + 4$.

\begin{eqnarray*}
\langle E \rangle	&	\stackrel{1}{\Rightarrow}	& \langle E \rangle + \langle T \rangle \\
						&	\stackrel{1}{\Rightarrow}	& \langle E \rangle + \langle T \rangle + \langle T \rangle \\
						&	\stackrel{2}{\Rightarrow}	& \langle T \rangle + \langle T \rangle + \langle T \rangle \\
						&	\stackrel{4}{\rightarrow}	& \langle P \rangle + \langle T \rangle + \langle T \rangle \\
						&	\stackrel{6}{\rightarrow}	& CONST_{1} + \langle T \rangle + \langle T \rangle \\
						&	\stackrel{3}{\rightarrow}	& CONST_{1} + \langle T \rangle \ast \langle P \rangle + \langle T \rangle \\
						&	\stackrel{6}{\rightarrow}	& CONST_{1} + CONST_{2} \ast \langle P \rangle + \langle T \rangle \\
						&	.	& \\
						&	.	&	\\
						&	.	&	\\
						&	\stackrel{*}{\rightarrow}	& CONST_{1} + CONST_{2} \ast CONST_{3} + CONST_{4} \\
\end{eqnarray*}

\begin{figure}[ht]

\psset{levelsep=15mm,nodesep=1mm}

\pstree{\TR{\nonterminal{E}}}{
	\pstree{\TR{\nonterminal{E}}}{
		\pstree{\TR{\nonterminal{E}}}{
			\pstree{\TR{\nonterminal{T}}}{
				\pstree{\TR{\nonterminal{P}}}{
					\TR{$Const_1$}
					\Tn
				}
			\Tn
			}
			\Tn
		}
		\TR{+}
		\pstree{\TR{\nonterminal{T}}}{
			\pstree{\TR{\nonterminal{T}}}{
				\pstree{\TR{\nonterminal{P}}}{
					\TR{$Const_2$}
					\Tn
				}
				\Tn
			}
			\TR{$\ast$}
			\pstree{\TR{\nonterminal{P}}}{
				\TR{$Const_3$}
				\Tn
			}
		}
	}
	\TR{$+$}
	\pstree{\TR{\nonterminal{T}}}{
		\Tn
		\pstree{\TR{\nonterminal{P}}}{
			\Tn
			\TR{$Const_4$}
		}
	}
}

\caption{Derivation Tree (Parse Tree)}

\end{figure}


LR Parsing: Scan input left to right and produce a reverse of the
rightmost % something - Ask irokie

\section*{Another Grammar for Arithmetic Expressions}

Consider

\begin{eqnarray}
\setcounter{equation}{1}
\langle E \rangle		& \to	& \langle E \rangle + \langle T \rangle \\
\langle E \rangle		& \to	& \langle T \rangle \\
\end{eqnarray}

\begin{eqnarray*}
\langle E \rangle	&	\stackrel{}{\Rightarrow}	&	\langle E \rangle + \langle T \rangle \\
						&	\stackrel{1}{\Rightarrow}	&	\langle E \rangle + \langle T \rangle + \langle T \rangle \\
						&	\stackrel{2}{\Rightarrow}	&	\langle T \rangle + \langle T \rangle + \langle T \rangle 
\end{eqnarray*}

\subsection*{Productions}

\begin{eqnarray}
\setcounter{equation}{1}
\langle E \rangle			& 	\to	& \langle T \rangle \langle E-List \rangle \\
\langle E-List \rangle	&	\to	& + \langle T \rangle \langle E-List \rangle \\
\langle E-List \rangle	&	\to	&	\epsilon 
\end{eqnarray}

\begin{eqnarray*}
\langle E \rangle	&	\Rightarrow	&	\langle T \rangle + \langle E-List \rangle \\
						&	\Rightarrow	&	\langle T \rangle + \langle T \rangle + \langle E-List \rangle \\
						&	\Rightarrow	&	\langle T \rangle + \langle T \rangle + \langle T \rangle \langle E-List \rangle \\ 
						&	\Rightarrow	&	\langle T \rangle + \langle T \rangle + \langle T \rangle 
\end{eqnarray*}

Consider

\begin{eqnarray}
\langle T \rangle	& 	\to	& \langle T \rangle \langle P \rangle \\
\langle T \rangle	&	\to	& \langle P \rangle \\
\end{eqnarray}

\begin{eqnarray*}
\langle T \rangle	&	\Rightarrow	&	\langle P \rangle \ast \langle P
\rangle \ast \langle P \rangle 
\end{eqnarray*}

\subsection*{The $E-Link$ Grammar}

\begin{eqnarray}
\setcounter{equation}{1}
\langle E \rangle			& 	\to	& \langle T \rangle \langle E-List \rangle \\
\langle E-List \rangle	&	\to	& + \langle T \rangle \langle E-List \rangle \\
\langle E-List \rangle	&	\to	& \epsilon \\
\langle T \rangle 		&	\to	& \langle P \rangle \langle T-List \rangle \\
\langle T-List \rangle	&	\to	& \ast \langle P \rangle \langle T-List \rangle \\
\langle P \rangle			&	\to	& \left( \langle E \rangle \right) \\
\langle P \rangle			&	\to	& COUNT
\end{eqnarray}

eg:

\begin{eqnarray*}
\langle T \rangle	&	\Rightarrow	&	\langle P \rangle \\
						&	\Rightarrow	&	\langle P \rangle \ast \langle P \rangle \langle T-List \rangle \\
						& 	\Rightarrow	& 	\langle P \rangle \ast \langle P \rangle \ast \langle P \rangle \ast \langle T-List \rangle \\
						&	\Rightarrow	&	\langle P \rangle \ast \langle P \rangle \ast \langle P \rangle \\ 
\end{eqnarray*}

\section*{Exercise}

\begin{eqnarray*}
\langle E \rangle	&	\stackrel{1}{\Rightarrow}	&	\langle T \rangle \langle E-List \rangle \\
						&	\stackrel{4}{\Rightarrow}	&	\langle P \rangle \langle T-List \rangle \langle E-List \rangle \\
						&	\stackrel{2}{\Rightarrow}	&	COUNT_{1} \langle T-List \rangle \langle E-List \rangle \\
						&	\stackrel{6}{\Rightarrow}	&	COUNT_{1} \langle E-List \rangle \\
						&	\stackrel{2}{\Rightarrow}	&	COUNT_{1} + \langle T \rangle \langle E-List \rangle \\
						&	\stackrel{6}{\Rightarrow}	&	COUNT_{1} + \langle P \rangle \langle T-List \rangle \langle E-List \rangle \\
						&	\stackrel{8}{\Rightarrow}	&	COUNT_{1} + COUNT_{2} \langle T-List \rangle \langle E-List \rangle \\
						&	\stackrel{ }{\Rightarrow}	&	COUNT_{1} + COUNT_{2} \ast \langle T-List \rangle \langle E-List \rangle \\
						&	.	&	\\
						&	.	&	\\
						&	.	&	\\
						&	\stackrel{ }{\Rightarrow}	&	COUNT_{1} + COUNT_{2} \ast COUNT_{3} \ast COUNT_{4}
\end{eqnarray*}

\begin{landscape}

\begin{figure}[ht]

\psset{levelsep=20mm,nodesep=0mm}

\pstree{\TR{\nonterminal{E}}}{
	\pstree{\TR{\nonterminal{T}}}{
		\pstree{\TR{\nonterminal{P}}}{
			\TR{$Const_{1}$}
			\Tn
		}
		\pstree{\TR{\nonterminal{T-List}}}{
			\TR{$\epsilon$}
			\Tn
		}
	}
	\pstree{\TR{\nonterminal{E-List}}}{
		\TR{$+$}
		\pstree{\TR{\nonterminal{T}}}{
			\pstree{\TR{\nonterminal{P}}}{
				\TR{$Const_{2}$}
				\Tn
			}
			\pstree{\TR{\nonterminal{T-List}}}{
				\TR{$\ast$}
				\pstree{\TR{\nonterminal{P}}}{
					\TR{$Const_{3}$}
					\Tn
				}
				\pstree{\TR{\nonterminal{T-List}}}{
					\Tn
					\TR{$\epsilon$}
				}
			}
		}
		\pstree{\TR{\nonterminal{E-List}}}{
			\Tn
			\TR{$+$}
			\pstree{\TR{\nonterminal{T}}}{
				\Tn
				\pstree{\TR{\nonterminal{P}}}{
					\TR{$Const_{4}$}
					\Tn
				}
				\pstree{\TR{\nonterminal{T-List}}}{
					\TR{$\epsilon$}
					\Tn
				}
				\Tn
			}
			\pstree{\TR{\nonterminal{E-List}}}{
				\TR{$\epsilon$}
				\Tn
			}
		}
	}
}

\caption{Derivation Tree}

\end{figure}

\end{landscape}

\end{document}
